theories/examples/enclaves/trusted_compute.v
@@ -16,7 +16,7 @@ Section sealed_42.
 
   Program Definition f42 : Addr := (finz.FinZ 42 eq_refl eq_refl).
   Definition sealed_42 : LWord → iProp Σ :=
-    λ w, (∃ b e v, ⌜finz.seq_between b e ## reserved_addresses⌝ ∗ ⌜w = LCap O b e f42 v⌝)%I.
+    λ w, (∃ b e v, ⌜w = LCap O b e f42 v⌝)%I.
   Definition sealed_42_ne : (leibnizO LWord) -n> (iPropO Σ) :=
       λne (w : leibnizO LWord), sealed_42 w%I.
 
